refactor of semantics + better ltac

GDS_Language.v
@@ -148,58 +148,69 @@ Definition interp_binop (b: BinopName) (n1 n2: nat) :=
   end.
 
 
-Fixpoint runStmtP (fuel: nat) (vg1: valuation) (vl1: valuation) (st: stmt): option (valuation * valuation) :=
+Fixpoint runStmt (fuel: nat) (vg: valuation) (vl: valuation) (st: stmt): option (valuation * valuation) :=
     match fuel with
     | O => None
     | S fuel' =>
         match st with
-        | varDeclStmt name e => match interp2 e vg1 vl1 with
-                                | Some n => Some (vg1, (vl1 $+ (name, varAss n)))
+        (*Interp expression, then assign it in local val*)
+        | varDeclStmt name e => match interp2 e vg vl with
+                                | Some n => Some (vg, (vl $+ (name, varAss n)))
                                 | None => None
                                 end
-        | ifStmt e s1 s2 => match interp2 e vg1 vl1 with
-                            | Some 0 => runStmtP fuel' vg1 vl1 s2
-                            | Some _n => runStmtP fuel' vg1 vl1 s1
+        (*If expr is >= 1, run s1, elsif 0 run s2, else crash*)
+        | ifStmt e s1 s2 => match interp2 e vg vl with
+                            | Some 0 => runStmt fuel' vg vl s2
+                            | Some _n => runStmt fuel' vg vl s1
                             | None => None
                             end
-        | whileStmt e s => match interp2 e vg1 vl1 with
-                            | Some 0 => Some (vg1, vl1)
-                            | Some _n => match (runStmtP fuel' vg1 vl1 s) with
-                                | Some (vgmid, vlmid) => runStmtP fuel' vgmid vlmid st
+        (*While e <> 0, run s, else skip*)
+        | whileStmt e s => match interp2 e vg vl with
+                            | Some 0 => Some (vg, vl)
+                            | Some _n => match (runStmt fuel' vg vl s) with
+                                | Some (vgmid, vlmid) => runStmt fuel' vgmid vlmid st
                                 | None => None
                                 end
                             | None => None
                             end
-        | assignmentStmt name e => match vl1 $? name with
-                                | Some _ => match interp2 e vg1 vl1 with
-                                    | Some n => Some (vg1, (vl1 $+ (name, varAss n)))
+        (*If name defined in local, reassign it with value of e, else do the same for global, else crash*)
+        | assignmentStmt name e => match vl $? name with
+                                | Some _ => match interp2 e vg vl with
+                                    | Some n => Some (vg, (vl $+ (name, varAss n)))
                                     | None => None
                                     end
-                                | None => match vg1 $? name with
-                                    | Some _ => match interp2 e vg1 vl1 with
-                                        | Some n => Some (vg1 $+ (name, varAss n), vl1)
+                                | None => match vg $? name with
+                                    | Some _ => match interp2 e vg vl with
+                                        | Some n => Some (vg $+ (name, varAss n), vl)
                                         | None => None
                                         end
                                     | None => None
                                     end
                                 end
-        | awaitStmt sig_name => Some (vg1, vl1)
+        (*Skip, await is checked in sequence, because await as last instruction does nothing anyways*)
+        | awaitStmt sig_name => Some (vg, vl)
+        (*If s1 is await:
+             check if the waited signal has been emitted. 
+                If so just run s2
+                else add waiting s2 to global valuation then skip, 
+        else just run s1 then s2*)
         | sequence s1 s2 => match s1 with
-            | awaitStmt sig_name => match interp (Var sig_name) vg1 with
-                | Some 0 | None => Some (vg1 $+ (("waiting_" ++ sig_name)%string, waitAss 1 s2), vl1)
-                | Some _n => runStmtP fuel' vg1 vl1 s2
+            | awaitStmt sig_name => match interp (Var sig_name) vg with
+                | Some 0 | None => Some (vg $+ (("waiting_" ++ sig_name)%string, waitAss 1 s2), vl)
+                | Some _n => runStmt fuel' vg vl s2
                 end
-            | _ => match runStmtP fuel' vg1 vl1 s1 with
-                | Some (vgmid, vlmid) => runStmtP fuel' vgmid vlmid s2
+            | _ => match runStmt fuel' vg vl s1 with
+                | Some (vgmid, vlmid) => runStmt fuel' vgmid vlmid s2
                 | None => None
                 end
             end
-        | assignCallMethodStmt ret method_name args => match vg1 $? method_name with
+        (*Get method, match arguments to parameters. If we want to assign the return value, read it in the local var of the executed func, then assign it*)
+        | assignCallMethodStmt ret method_name args => match vg $? method_name with
             | Some (methodAss name_args found_ret found_body) => match 
-                (runStmtP fuel' vg1 
+                (runStmt fuel' vg 
                 (fold_left 
                     (fun (acc: valuation) (arg_argname: expr * string) => 
-                        match interp2 (fst arg_argname) vg1 vl1 with
+                        match interp2 (fst arg_argname) vg vl with
                         | Some n => (acc $+ ((snd arg_argname), varAss n))
                         (*If we give an argument that isn't defined, it is not added to the valuation.
                         this might not be the correct behavior (would be better if the whole runStmt returned None. TODO: investigate)*)
@@ -210,26 +221,27 @@ Fixpoint runStmtP (fuel: nat) (vg1: valuation) (vl1: valuation) (st: stmt): opti
                 found_body) with
                 | Some (vgmid, vlmid) => match ret, found_ret with
                     | Some s_ret, Some s_found_ret => match interp (Var s_found_ret) vlmid with
-                        | Some r => match runStmtP fuel' vgmid vl1 (assignmentStmt s_ret (Const r)) with
+                        | Some r => match runStmt fuel' vgmid vl (assignmentStmt s_ret (Const r)) with
                             | Some (vg2, vl2) => Some (vg2, vl2)
-                            | None => Some (vgmid, vl1 $+ (s_ret, varAss r))
+                            | None => Some (vgmid, vl $+ (s_ret, varAss r))
                             end
                         | None => None 
                         end
                     (*Assigning void to a var*)
                     | Some _, None => None
                     (*Not reading the return of a non-void func*)
-                    | None, _ => Some (vgmid, vl1)
+                    | None, _ => Some (vgmid, vl)
                     end
                 | None => None
                 end
             | _ => None
             end
-        | emitSignalStmt sig_name opt_callback args => let vgmid := (vg1 $+ (sig_name, varAss 1)) in match opt_callback with
-            | Some (f, _n) => match runStmtP fuel' vgmid vl1 (assignCallMethodStmt None f args) with
+        (*Mark signal as emitted, check for callback (if exists, call this function with args of signal), then check for awaiting body (if exists, call this function)*)
+        | emitSignalStmt sig_name opt_callback args => let vgmid := (vg $+ (sig_name, varAss 1)) in match opt_callback with
+            | Some (f, _n) => match runStmt fuel' vgmid vl (assignCallMethodStmt None f args) with
                 | Some (vgmid', vlmid') => match vgmid' $? ("waiting_" ++ sig_name)%string with
                     (*Here we do a mini context switch for the local val*)
-                    | Some (waitAss _ body) => match runStmtP fuel' vgmid' $0 body with
+                    | Some (waitAss _ body) => match runStmt fuel' vgmid' $0 body with
                         | Some (vg2, vl2) => Some (vg2, vlmid')
                         | None => None
                         end
@@ -238,34 +250,39 @@ Fixpoint runStmtP (fuel: nat) (vg1: valuation) (vl1: valuation) (st: stmt): opti
                 | None => None
                 end
             | None => match vgmid $? ("waiting_" ++ sig_name)%string with
-                | Some (waitAss _ body) => runStmtP fuel' vgmid vl1 body
-                | _ => Some (vgmid, vl1)
+                | Some (waitAss _ body) => runStmt fuel' vgmid vl body
+                | _ => Some (vgmid, vl)
                 end
             end
-        | skip => Some (vg1, vl1)
+        | skip => Some (vg, vl)
         end
     end.
 
-Fixpoint runP (fuel: nat) (v: valuation) (d: topLevelDecl) : option valuation :=
+Fixpoint run (fuel: nat) (v: valuation) (d: topLevelDecl) : option valuation :=
     match fuel with
     | O => None
     | S fuel' =>
         match d with
+        (*Same as for runStmt*)
         | classVarDecl name e => match (interp e v) with
                                 | Some n => Some (v $+ (name, varAss n))
                                 | None => None
                                 end
+        (*Just add method to valuation*)
         | methodDecl name args ret body => Some (v $+ (name, methodAss args ret body))
-        | readyDecl body => match (runStmtP fuel' v ($0) body) with
+        (*Run the ready func once*)
+        | readyDecl body => match (runStmt fuel' v ($0) body) with
             | Some (vg2, vl2) => Some vg2
             | None => None
             end
-        | processDecl body => if (Nat.eqb fuel' 1) then Some v else match runStmtP fuel' v $0 body with
-            | Some (vgmid, vlmid) => runP fuel' vgmid d
+        (*Run until no fuel remaining*)
+        | processDecl body => if (Nat.eqb fuel' 1) then Some v else match runStmt fuel' v $0 body with
+            | Some (vgmid, vlmid) => run fuel' vgmid d
             | None => None
             end
-        | SequenceDecl d1 d2 => match runP fuel' v d1 with
-            | Some vmid => runP fuel' vmid d2
+        (*Run d1 then d2*)
+        | SequenceDecl d1 d2 => match run fuel' v d1 with
+            | Some vmid => run fuel' vmid d2
             | None => None
             end
         | EndDecl => Some v
@@ -273,7 +290,7 @@ Fixpoint runP (fuel: nat) (v: valuation) (d: topLevelDecl) : option valuation :=
     end.
 
 
-Fixpoint runStmtDualP (fuel: nat) (vg : valuation * valuation) (vl: valuation) (st: stmt) : option((valuation * valuation) * valuation) :=
+Fixpoint runStmtDual (fuel: nat) (vg : valuation * valuation) (vl: valuation) (st: stmt) : option((valuation * valuation) * valuation) :=
     match fuel with
     | O => None
     | S fuel' => match interp (Var "current") (fst vg) with
@@ -283,14 +300,14 @@ Fixpoint runStmtDualP (fuel: nat) (vg : valuation * valuation) (vl: valuation) (
                 | None => None
                 end
             | ifStmt e s1 s2 => match interp2 e (fst vg) vl with
-                | Some 0 => runStmtDualP fuel' vg vl s2
-                | Some _n => runStmtDualP fuel' vg vl s1
+                | Some 0 => runStmtDual fuel' vg vl s2
+                | Some _n => runStmtDual fuel' vg vl s1
                 | None => None
                 end
             | whileStmt e s => match interp2 e (fst vg) vl with
                 | Some 0 => Some (vg, vl)
-                | Some _n => match runStmtDualP fuel' vg vl s with
-                    | Some (vgmid, vlmid) => runStmtDualP fuel' vgmid vlmid st
+                | Some _n => match runStmtDual fuel' vg vl s with
+                    | Some (vgmid, vlmid) => runStmtDual fuel' vgmid vlmid st
                     | None => None
                     end
                 | None => None
@@ -313,16 +330,16 @@ Fixpoint runStmtDualP (fuel: nat) (vg : valuation * valuation) (vl: valuation) (
                 | awaitStmt sig_name => match interp (Var sig_name) (fst vg) with
                     (*Here, we add "waiting" to fst and snd of vg, but fst is probably sufficient*)
                     | Some 0 | None => Some (((fst vg) $+ (("waiting_" ++ sig_name)%string, waitAss 1 s2), (snd vg) $+ (("waiting_" ++ sig_name)%string, waitAss 1 s2)), vl)
-                    | Some _n => runStmtDualP fuel' vg vl s2
+                    | Some _n => runStmtDual fuel' vg vl s2
                     end
-                | _ => match runStmtDualP fuel' vg vl s1 with
-                    | Some (vgmid, vlmid) => runStmtDualP fuel' vgmid vlmid s2
+                | _ => match runStmtDual fuel' vg vl s1 with
+                    | Some (vgmid, vlmid) => runStmtDual fuel' vgmid vlmid s2
                     | None => None
                     end
                 end
             | assignCallMethodStmt ret method_name args => match (fst vg) $? method_name with
                 | Some (methodAss name_args found_ret found_body) => match
-                    (runStmtDualP fuel' vg
+                    (runStmtDual fuel' vg
                     (fold_left
                         (fun (acc: valuation) (arg_argname: expr * string) =>
                             match interp2 (fst arg_argname) (fst vg) vl with
@@ -334,7 +351,7 @@ Fixpoint runStmtDualP (fuel: nat) (vg : valuation * valuation) (vl: valuation) (
                                 found_body) with
                         | Some (vgmid, vlmid) => match ret, found_ret with
                             | Some s_ret, Some s_found_ret => match interp (Var s_found_ret) vlmid with
-                                | Some r => match runStmtDualP fuel' vgmid vl (assignmentStmt s_ret (Const r)) with
+                                | Some r => match runStmtDual fuel' vgmid vl (assignmentStmt s_ret (Const r)) with
                                     | Some (vg2, vl2) => Some (vg2, vl2)
                                     | None => Some (vgmid, vl $+ (s_ret, varAss r))
                                     end
@@ -351,15 +368,15 @@ Fixpoint runStmtDualP (fuel: nat) (vg : valuation * valuation) (vl: valuation) (
                 end
             | emitSignalStmt sig_name opt_callback args => let vgmid := ((fst vg) $+ (sig_name, varAss 1), (snd vg) $+ (sig_name, varAss 1)) in match opt_callback with
             (*Context switch if n = 2*)
-                | Some (f, 1) => match runStmtDualP fuel' vgmid vl (assignCallMethodStmt None f args) with
+                | Some (f, 1) => match runStmtDual fuel' vgmid vl (assignCallMethodStmt None f args) with
                     | Some (vgmid', vlmid') => match (fst vgmid') $? ("waiting_" ++ sig_name)%string with
                         (*Context switch if 2*)
-                        | Some (waitAss 1 body) => match runStmtDualP fuel' vgmid' $0 body with
+                        | Some (waitAss 1 body) => match runStmtDual fuel' vgmid' $0 body with
                             | Some (vg2, vl2) => Some (vg2, vlmid')
                             | None => None
                             end
                         (*Double checking: here we want to set current to 2, call body with an empty local val, set current to 1 again and return that new global val with the old local one*)
-                        | Some (waitAss 2 body) => let vgswitch := ((fst vgmid') $+ (("current")%string, varAss 2), snd vgmid') in match runStmtDualP fuel' vgswitch $0 body with
+                        | Some (waitAss 2 body) => let vgswitch := ((fst vgmid') $+ (("current")%string, varAss 2), snd vgmid') in match runStmtDual fuel' vgswitch $0 body with
                             | Some (vg2, vl2) => Some (((fst vg2) $+ (("current")%string, varAss 1) , snd vg2), vlmid')
                             | None => None
                             end
@@ -368,14 +385,14 @@ Fixpoint runStmtDualP (fuel: nat) (vg : valuation * valuation) (vl: valuation) (
                     | None => None
                     end
                 (*NB: there is a world where this is wrong because we context switch but still keep the same local val, which we return later after switching back*)
-                | Some (f, 2) => let vgswitch := ((fst vgmid) $+ (("current")%string, varAss 2), snd vgmid) in match runStmtDualP fuel' vgswitch vl (assignCallMethodStmt None f args) with
+                | Some (f, 2) => let vgswitch := ((fst vgmid) $+ (("current")%string, varAss 2), snd vgmid) in match runStmtDual fuel' vgswitch vl (assignCallMethodStmt None f args) with
                     | Some (vgmid', vlmid') => match (fst vgmid') $? ("waiting_" ++ sig_name)%string with
                         (*Already switched, so stay in current if two or switch back if 1*)
-                        | Some (waitAss 1 body) => let vgswitch' := ((fst vgmid') $+ (("current")%string, varAss 1), snd vgmid') in match runStmtDualP fuel' vgswitch' $0 body with
+                        | Some (waitAss 1 body) => let vgswitch' := ((fst vgmid') $+ (("current")%string, varAss 1), snd vgmid') in match runStmtDual fuel' vgswitch' $0 body with
                             | Some (vg2, vl2) => Some (vg2, vlmid')
                             | None => None
                             end
-                        | Some (waitAss 2 body) => match runStmtDualP fuel' vgmid' $0 body with
+                        | Some (waitAss 2 body) => match runStmtDual fuel' vgmid' $0 body with
                             | Some (vg2, vl2) => Some (((fst vg2) $+ (("current")%string, varAss 1) , snd vg2), vlmid')
                             | None => None
                             end
@@ -386,11 +403,11 @@ Fixpoint runStmtDualP (fuel: nat) (vg : valuation * valuation) (vl: valuation) (
                     end
                 | None => match (fst vgmid) $? ("waiting_" ++ sig_name)%string with
                     (*Context switch if 2*)
-                    | Some (waitAss 1 body) => match runStmtDualP fuel' vgmid $0 body with
+                    | Some (waitAss 1 body) => match runStmtDual fuel' vgmid $0 body with
                         | Some (vg2, vl2) => Some (vg2, vl)
                         | None => None
                         end
-                    | Some (waitAss 2 body) => let vgswitch := ((fst vgmid) $+ (("current")%string, varAss 2), snd vgmid) in match runStmtDualP fuel' vgswitch $0 body with
+                    | Some (waitAss 2 body) => let vgswitch := ((fst vgmid) $+ (("current")%string, varAss 2), snd vgmid) in match runStmtDual fuel' vgswitch $0 body with
                         | Some (vg2, vl2) => Some (((fst vg2) $+ (("current")%string, varAss 1) , snd vg2), vl)
                         | None => None
                         end
@@ -406,14 +423,14 @@ Fixpoint runStmtDualP (fuel: nat) (vg : valuation * valuation) (vl: valuation) (
                 | None => None
                 end
             | ifStmt e s1 s2 => match interp2 e (snd vg) vl with
-                | Some 0 => runStmtDualP fuel' vg vl s2
-                | Some _n => runStmtDualP fuel' vg vl s1
+                | Some 0 => runStmtDual fuel' vg vl s2
+                | Some _n => runStmtDual fuel' vg vl s1
                 | None => None
                 end
             | whileStmt e s => match interp2 e (snd vg) vl with
                 | Some 0 => Some (vg, vl)
-                | Some _n => match runStmtDualP fuel' vg vl s with
-                    | Some (vgmid, vlmid) => runStmtDualP fuel' vgmid vlmid st
+                | Some _n => match runStmtDual fuel' vg vl s with
+                    | Some (vgmid, vlmid) => runStmtDual fuel' vgmid vlmid st
                     | None => None
                     end
                 | None => None
@@ -436,16 +453,16 @@ Fixpoint runStmtDualP (fuel: nat) (vg : valuation * valuation) (vl: valuation) (
                 | awaitStmt sig_name => match interp (Var sig_name) (fst vg) with
                     (*Here, we add "waiting" to fst and snd of vg, but fst is probably sufficient*)
                     | Some 0 | None => Some (((fst vg) $+ (("waiting_" ++ sig_name)%string, waitAss 2 s2), (snd vg) $+ (("waiting_" ++ sig_name)%string, waitAss 2 s2)), vl)
-                    | Some _n => runStmtDualP fuel' vg vl s2
+                    | Some _n => runStmtDual fuel' vg vl s2
                     end
-                | _ => match runStmtDualP fuel' vg vl s1 with
-                    | Some (vgmid, vlmid) => runStmtDualP fuel' vgmid vlmid s2
+                | _ => match runStmtDual fuel' vg vl s1 with
+                    | Some (vgmid, vlmid) => runStmtDual fuel' vgmid vlmid s2
                     | None => None
                     end
                 end
             | assignCallMethodStmt ret method_name args => match (snd vg) $? method_name with
                 | Some (methodAss name_args found_ret found_body) => match
-                    (runStmtDualP fuel' vg
+                    (runStmtDual fuel' vg
                     (fold_left
                         (fun (acc: valuation) (arg_argname: expr * string) =>
                             match interp2 (fst arg_argname) (snd vg) vl with
@@ -457,7 +474,7 @@ Fixpoint runStmtDualP (fuel: nat) (vg : valuation * valuation) (vl: valuation) (
                                 found_body) with
                         | Some (vgmid, vlmid) => match ret, found_ret with
                             | Some s_ret, Some s_found_ret => match interp (Var s_found_ret) vlmid with
-                                | Some r => match runStmtDualP fuel' vgmid vl (assignmentStmt s_ret (Const r)) with
+                                | Some r => match runStmtDual fuel' vgmid vl (assignmentStmt s_ret (Const r)) with
                                     | Some (vg2, vl2) => Some (vg2, vl2)
                                     | None => Some (vgmid, vl $+ (s_ret, varAss r))
                                     end
@@ -475,14 +492,14 @@ Fixpoint runStmtDualP (fuel: nat) (vg : valuation * valuation) (vl: valuation) (
             | emitSignalStmt sig_name opt_callback args => let vgmid := ((fst vg) $+ (sig_name, varAss 1), (snd vg) $+ (sig_name, varAss 1)) in match opt_callback with
             (*Context switch if n = 1*)
                 (*NB: there is a world where this is wrong because we context switch but still keep the same local val, which we return later after switching back*)
-                | Some (f, 1) => let vgswitch := ((fst vgmid) $+ (("current")%string, varAss 1), snd vgmid) in match runStmtDualP fuel' vgswitch vl (assignCallMethodStmt None f args) with
+                | Some (f, 1) => let vgswitch := ((fst vgmid) $+ (("current")%string, varAss 1), snd vgmid) in match runStmtDual fuel' vgswitch vl (assignCallMethodStmt None f args) with
                     | Some (vgmid', vlmid') => match (fst vgmid') $? ("waiting_" ++ sig_name)%string with
                         (*Already switched, so stay in current if 1 or switch back if 2*)
-                        | Some (waitAss 1 body) => match runStmtDualP fuel' vgmid' $0 body with
+                        | Some (waitAss 1 body) => match runStmtDual fuel' vgmid' $0 body with
                             | Some (vg2, vl2) => Some (((fst vg2) $+ (("current")%string, varAss 2) , snd vg2), vlmid')
                             | None => None
                             end
-                        | Some (waitAss 2 body) => let vgswitch' := ((fst vgmid') $+ (("current")%string, varAss 2), snd vgmid') in match runStmtDualP fuel' vgswitch' $0 body with
+                        | Some (waitAss 2 body) => let vgswitch' := ((fst vgmid') $+ (("current")%string, varAss 2), snd vgmid') in match runStmtDual fuel' vgswitch' $0 body with
                             | Some (vg2, vl2) => Some (vg2, vlmid')
                             | None => None
                             end
@@ -491,15 +508,15 @@ Fixpoint runStmtDualP (fuel: nat) (vg : valuation * valuation) (vl: valuation) (
                         end
                     | None => None
                     end
-                | Some (f, 2) => match runStmtDualP fuel' vgmid vl (assignCallMethodStmt None f args) with
+                | Some (f, 2) => match runStmtDual fuel' vgmid vl (assignCallMethodStmt None f args) with
                     | Some (vgmid', vlmid') => match (fst vgmid') $? ("waiting_" ++ sig_name)%string with
                         (*Context switch if 1*)
                         (*Double checking: here we want to set current to 1, call body with an empty local val, set current to 2 again and return that new global val with the old local one*)
-                        | Some (waitAss 1 body) => let vgswitch := ((fst vgmid') $+ (("current")%string, varAss 1), snd vgmid') in match runStmtDualP fuel' vgswitch $0 body with
+                        | Some (waitAss 1 body) => let vgswitch := ((fst vgmid') $+ (("current")%string, varAss 1), snd vgmid') in match runStmtDual fuel' vgswitch $0 body with
                             | Some (vg2, vl2) => Some (((fst vg2) $+ (("current")%string, varAss 2) , snd vg2), vlmid')
                             | None => None
                             end
-                        | Some (waitAss 2 body) => match runStmtDualP fuel' vgmid' $0 body with
+                        | Some (waitAss 2 body) => match runStmtDual fuel' vgmid' $0 body with
                             | Some (vg2, vl2) => Some (vg2, vlmid')
                             | None => None
                             end
@@ -509,11 +526,11 @@ Fixpoint runStmtDualP (fuel: nat) (vg : valuation * valuation) (vl: valuation) (
                     end
                 | None => match (fst vgmid) $? ("waiting_" ++ sig_name)%string with
                     (*Context switch if 1*)
-                    | Some (waitAss 1 body) => let vgswitch := ((fst vgmid) $+ (("current")%string, varAss 1), snd vgmid) in match runStmtDualP fuel' vgswitch $0 body with
+                    | Some (waitAss 1 body) => let vgswitch := ((fst vgmid) $+ (("current")%string, varAss 1), snd vgmid) in match runStmtDual fuel' vgswitch $0 body with
                         | Some (vg2, vl2) => Some (((fst vg2) $+ (("current")%string, varAss 2) , snd vg2), vl)
                         | None => None
                         end
-                    | Some (waitAss 2 body) => match runStmtDualP fuel' vgmid $0 body with
+                    | Some (waitAss 2 body) => match runStmtDual fuel' vgmid $0 body with
                         | Some (vg2, vl2) => Some (vg2, vl)
                         | None => None
                         end
@@ -527,8 +544,9 @@ Fixpoint runStmtDualP (fuel: nat) (vg : valuation * valuation) (vl: valuation) (
         end
     end.
 
+
 (*For this to be correct, the initial val should have current as 1 in fst v*)
-Fixpoint runDualP (fuel: nat) (v : valuation * valuation) (dA: topLevelDecl) (dB: topLevelDecl) : option (valuation * valuation) :=
+Fixpoint runDual (fuel: nat) (v : valuation * valuation) (dA: topLevelDecl) (dB: topLevelDecl) : option (valuation * valuation) :=
     match fuel with
     | O => None
     | S fuel' => match interp (Var "current") (fst v) with
@@ -538,39 +556,39 @@ Fixpoint runDualP (fuel: nat) (v : valuation * valuation) (dA: topLevelDecl) (dB
                 | None => None
                 end
             | methodDecl name args ret body => Some ((fst v) $+ (name, methodAss args ret body), snd v)
-            | readyDecl body => match (runStmtDualP fuel' v $0 body) with
+            | readyDecl body => match (runStmtDual fuel' v $0 body) with
                 | Some (vg2, vl2) => Some vg2
                 | None => None
                 end
             | processDecl bodyA => if (Nat.eqb fuel' 1) then Some v else match dB with
                 (*Run both processes one after the other until no fuel, in which case we return the last val*)
-                | processDecl bodyB => match runStmtDualP fuel' v $0 bodyA with
-                    | Some (vgmid, vlmid) => let vgswitch := ((fst vgmid) $+ (("current")%string, varAss 2), snd vgmid) in match runStmtDualP fuel' vgswitch $0 bodyB with
-                        | Some (vg2, vl2) => let vgswitch' := ((fst vg2) $+ (("current")%string, varAss 1), snd vg2) in runDualP fuel' vgswitch' dA dB
+                | processDecl bodyB => match runStmtDual fuel' v $0 bodyA with
+                    | Some (vgmid, vlmid) => let vgswitch := ((fst vgmid) $+ (("current")%string, varAss 2), snd vgmid) in match runStmtDual fuel' vgswitch $0 bodyB with
+                        | Some (vg2, vl2) => let vgswitch' := ((fst vg2) $+ (("current")%string, varAss 1), snd vg2) in runDual fuel' vgswitch' dA dB
                         | None => None
                         end
                     | None => None
                     end
                 (*B is over, but might still be waiting or have a function callback in a signal of A, runStmt prog A then rerun*)
-                | EndDecl => match runStmtDualP fuel' v $0 bodyA with
-                    | Some (vgmid, vlmid) => runDualP fuel' vgmid dA dB
+                | EndDecl => match runStmtDual fuel' v $0 bodyA with
+                    | Some (vgmid, vlmid) => runDual fuel' vgmid dA dB
                     | None => None
                     end
                 (*If B is not over but not process, switch and rerun*)
-                | _ => let vgswitch := (((fst v) $+ (("current")%string, varAss 2)), snd v) in runDualP fuel' vgswitch dA dB
+                | _ => let vgswitch := (((fst v) $+ (("current")%string, varAss 2)), snd v) in runDual fuel' vgswitch dA dB
                 end
-            | SequenceDecl d1 d2 => match runDualP fuel' v d1 dB with
-                | Some vmid => runDualP fuel' vmid d2 dB
+            | SequenceDecl d1 d2 => match runDual fuel' v d1 dB with
+                | Some vmid => runDual fuel' vmid d2 dB
                 | None => None
                 end
             (*If B process, runStmt B then rerun. If B = endDecl, done. Else, just run B*)
             | EndDecl => match dB with
-                | processDecl bodyB => let vgswitch := (((fst v) $+ (("current")%string, varAss 2)), snd v) in match runStmtDualP fuel' vgswitch $0 bodyB with
-                    | Some (vg2, vl2) => let vgswitch' := ((fst vg2) $+ (("current")%string, varAss 1), snd vg2) in runDualP fuel' vgswitch' dA dB
+                | processDecl bodyB => let vgswitch := (((fst v) $+ (("current")%string, varAss 2)), snd v) in match runStmtDual fuel' vgswitch $0 bodyB with
+                    | Some (vg2, vl2) => let vgswitch' := ((fst vg2) $+ (("current")%string, varAss 1), snd vg2) in runDual fuel' vgswitch' dA dB
                     | None => None
                     end
                 | EndDecl => Some v
-                | _ => let vgswitch := (((fst v) $+ (("current")%string, varAss 2)), snd v) in runDualP fuel' vgswitch dA dB
+                | _ => let vgswitch := (((fst v) $+ (("current")%string, varAss 2)), snd v) in runDual fuel' vgswitch dA dB
                 end
             end
         | Some 2 => match dB with
@@ -579,252 +597,19 @@ Fixpoint runDualP (fuel: nat) (v : valuation * valuation) (dA: topLevelDecl) (dB
                 | None => None
                 end
             | methodDecl name args ret body => Some (fst v, (snd v) $+ (name, methodAss args ret body))
-            | readyDecl body => match (runStmtDualP fuel' v $0 body) with
+            | readyDecl body => match (runStmtDual fuel' v $0 body) with
                 | Some (vg2, vl2) => Some vg2
                 | None => None
                 end
             (*Switch and rerun*)
-            | processDecl _ => let vgswitch := (((fst v) $+ (("current")%string, varAss 1)), snd v) in runDualP fuel' vgswitch dA dB
-            | SequenceDecl d1 d2 => match runDualP fuel' v dA d1 with
-                | Some vmid => runDualP fuel' vmid dA d2
+            | processDecl _ => let vgswitch := (((fst v) $+ (("current")%string, varAss 1)), snd v) in runDual fuel' vgswitch dA dB
+            | SequenceDecl d1 d2 => match runDual fuel' v dA d1 with
+                | Some vmid => runDual fuel' vmid dA d2
                 | None => None
                 end
             (*Switch and rerun*)
-            | EndDecl => let vgswitch := (((fst v) $+ (("current")%string, varAss 1)), snd v) in runDualP fuel' vgswitch dA dB
+            | EndDecl => let vgswitch := (((fst v) $+ (("current")%string, varAss 1)), snd v) in runDual fuel' vgswitch dA dB
             end
         | _ => None
         end
     end.
-
-(* 
-Fixpoint runStmt (fuel: nat) (vg1: valuation) (vl1: valuation) (st: stmt) (vg2: valuation) (vl2: valuation): Prop :=
-    match fuel with
-    | O => False
-    | S fuel' => 
-        match st with
-        (* check what we're gonna write with interp2 and assign local var *)
-        | varDeclStmt s e => exists n, n = interp2 e vg1 vl1  /\ vl2 = (vl1 $+ (s, varAss n)) /\ vg2 = vg1
-        | ifStmt e s1 s2 => (exists r, r = interp2 e vg1 vl1 /\ r <> 0 /\ runStmt fuel' vg1 vl1 s1 vg2 vl2) \/
-            (0 = interp2 e vg1 vl1 /\ runStmt fuel' vg1 vl1 s2 vg2 vl2)
-        | whileStmt e s => (exists r vgmid vlmid, r = interp2 e vg1 vl1 /\ r <> 0 /\ runStmt fuel' vg1 vl1 s vgmid vlmid
-            /\ runStmt fuel' vgmid vlmid st vg2 vl2) \/ (0 = interp2 e vg1 vl1 /\ vg1 = vg2 /\ vl1 = vl2)
-        (*Check local val, if exists, reassign, else check global, if exists reassign, else crash (prop is false)*)
-        | assignmentStmt s e => (vl1 $? s <> None /\ exists n, n = interp2 e vg1 vl1 /\ vl2 = (vl1 $+ (s, varAss n)) /\ vg1 = vg2) \/
-            (vg1 $? s <> None /\ vl1 $? s = None /\ exists n, n = interp2 e vg1 vl1 /\ vg2 = (vg1 $+ (s, varAss n)) /\ vl1 = vl2)
-        (*We check awaits in Seqs, so if we reach this case, it is either the only instruction in the program or the last one, either way it does nothing*)
-        | awaitStmt sig_name => vg1 = vg2 /\ vl1 = vl2
-        | sequence s1 s2 => match s1 with
-            (*If we want to await a signal, we check if it has been emitted yet or no. If yes, we continue as a normal Seq,
-            else, we add a waiting assignment to the valuation with the body of the Seq, which will be checked when the signal is emitted*)
-            | awaitStmt sig_name => (exists r, (interp (Var sig_name) vg1) = r /\ r <> 0 /\ runStmt fuel' vg1 vl1 s2 vg2 vl2) \/ 
-            ((interp (Var sig_name) vg1 = 0) /\ vg2 = (vg1 $+ (("waiting_" ++ sig_name)%string, waitAss 1 s2)) /\ vl1 = vl2)
-            | _ => exists vgmid vlmid, runStmt fuel' vg1 vl1 s1 vgmid vlmid /\ runStmt fuel' vgmid vlmid s2 vg2 vl2
-            end
-        | assignCallMethodStmt ret method_name args =>
-            exists name_args found_ret found_body, vg1 $? method_name = 
-            Some (methodAss name_args found_ret found_body) /\
-                exists vlmid vgmid,
-                runStmt fuel' vg1 
-                (fold_left 
-                    (fun (acc: valuation) (arg_argname: expr * string) => 
-                        (acc $+ ((snd arg_argname), varAss (interp2 (fst arg_argname) vg1 vl1)))
-                    ) 
-                    (combine args name_args) ($0)) 
-                found_body vgmid vlmid
-                /\ match ret, found_ret with
-                    | Some s_ret, Some s_found_ret => 
-                        (exists r, interp (Var s_found_ret) vlmid = r 
-                        /\ 
-                        ((runStmt fuel' vgmid vl1 (assignmentStmt s_ret (Const r)) vg2 vl2) (* if already defined (locally or globally), reassign to new value r *)
-                        \/
-                        vl1 $? s_ret = None /\ vgmid $? s_ret = None /\ (vl2 = vl1 $+ (s_ret, varAss r) /\ vgmid = vg2 (* otw, new val *)
-                        )))
-                    | Some _, None => False
-                    | None, _ => vl2 = vl1 /\ vg2 = vgmid
-                    end
-        (*If callback is Some, assignCallMethodStmt in garbage return variable with args.
-        If None, do nothing. In both cases, set the signal to true in valuation to show it has been emitted.
-        Check if a function is waiting for the signal. If so, call it after the callback but before resuming execution*)
-        | emitSignalStmt sig_name opt_callback args => exists vgmid vgmid' vlmid', vgmid = (vg1 $+ (sig_name, varAss 1)) /\
-            match opt_callback with
-                | Some (f, n) => runStmt fuel' vgmid vl1 (assignCallMethodStmt None f args) vgmid' vlmid'
-                | None => vgmid = vgmid' /\ vl1 = vlmid'
-                end /\ match vgmid' $? ("waiting_" ++ sig_name)%string with
-                    | Some (waitAss _ b) => runStmt fuel' vgmid' vlmid' b vg2 vl2
-                    | _ => vgmid' = vg2 /\ vlmid' = vl2
-                    end
-        | skip => vg1 = vg2 /\ vl1 = vl2
-        end
-    end.
-
-
-Fixpoint run (fuel: nat) (v1: valuation) (d: topLevelDecl) (v2: valuation): Prop:=
-    match fuel with
-    | O => False
-    | S fuel' =>
-        match d with
-        | classVarDecl s e => exists n, n = interp e v1  /\ v2 = (v1 $+ (s, varAss n))
-        | methodDecl s l ret st => v2 = (v1 $+ (s, methodAss l ret st))
-        | readyDecl st => (*stmt ->*) exists vl2, runStmt fuel' v1 ($0) st v2 vl2 (*TODO: voir cette histoire de stmt -> *)
-        | processDecl st => (* stmt ->  *) exists v' vl2, runStmt fuel' v1 $0 st v' vl2  /\ run fuel' v' d v2   
-        | SequenceDecl d1 d2 => exists vmid, run fuel' v1 d1 vmid /\ run fuel' vmid d2 v2 
-        | EndDecl => v1 = v2
-        end 
-    end.
-
-
- Fixpoint runStmtDual (fuel: nat) (vg1: valuation * valuation) (vl1: valuation) (st: stmt) (vg2: valuation * valuation) (vl2: valuation): Prop :=
-     match fuel with
-    | O => False
-    | S fuel' => match interp (Var "current") (fst vg1) with
-        | 1 =>  match st with
-            | varDeclStmt s e => exists n, n = interp2 e (fst vg1) vl1  /\ vl2 = (vl1 $+ (s, varAss n)) /\ vg1 = vg2 
-            | ifStmt e s1 s2 => (exists r, r = interp2 e (fst vg1) vl1 /\ r <> 0 /\ runStmtDual fuel' vg1 vl1 s1 vg2 vl2) \/
-                (0 = interp2 e (fst vg1) vl1 /\ runStmtDual fuel' vg1 vl1 s2 vg2 vl2)
-            | whileStmt e s => (exists r vgmid vlmid, r = interp2 e (fst vg1) vl1 /\ r <> 0 /\ runStmtDual fuel' vg1 vl1 s vgmid vlmid 
-                /\ runStmtDual fuel' vgmid vlmid st vg2 vl2) \/ (0 = interp2 e (fst vg1) vl1 /\ vg1 = vg2 /\ vl1 = vl2)
-            (*Check local val, if exists, reassign, else check global, if exists reassign, else crash (prop is false)*)
-            | assignmentStmt s e => (vl1 $? s <> None /\ exists n, n = interp2 e (fst vg1) vl1 /\ vl2 = (vl1 $+ (s, varAss n)) /\ vg1 = vg2) \/
-                ((fst vg1) $? s <> None /\ vl1 $? s = None /\ exists n, n = interp2 e (fst vg1) vl1 /\ vg2 = ((fst vg1) $+ (s, varAss n), snd vg1) /\ vl1 = vl2)
-            | awaitStmt sig_name => vg1 = vg2 /\ vl1 = vl2
-            | sequence s1 s2 => match s1 with
-                | awaitStmt sig_name => (exists r, (interp (Var sig_name) (fst vg1)) = r  /\ r <> 0 /\ runStmtDual fuel' vg1 vl1 s2 vg2 vl2) \/ 
-                ((interp (Var sig_name) (fst vg1) = 0) /\ vg2 = (((fst vg1) $+ (("waiting_" ++ sig_name)%string, waitAss 1 s2)), ((snd vg1) $+ (("waiting_" ++ sig_name)%string, waitAss 1 s2)))
-                /\ vl1 = vl2)
-                | _ => exists vgmid vlmid, runStmtDual fuel' vg1 vl1 s1 vgmid vlmid /\ runStmtDual fuel' vgmid vlmid s2 vg2 vl2
-                end
-            | assignCallMethodStmt ret method_name args =>
-                match (fst vg1) $? method_name with 
-                | Some (methodAss name_args found_ret found_body) => 
-                    exists vlmid,
-                    runStmtDual fuel' vg1
-                    (fold_left 
-                        (fun (acc: valuation) (arg_argname: expr * string) => 
-                            (acc $+ ((snd arg_argname), varAss (interp2 (fst arg_argname) (fst vg1) vl1)))
-                        ) 
-                        (combine args name_args) ($0)) 
-                    found_body vg2 vlmid
-                    /\ match ret, found_ret with
-                        | Some s_ret, Some s_found_ret =>  (exists r, interp (Var s_found_ret) vlmid = r /\ vl2 = vl1 $+ (s_ret, varAss r))
-                        | Some _, None => False
-                        | None, _ => vl2 = vlmid
-                        end    
-                | _ => False
-                end
-            | emitSignalStmt sig_name opt_callback args => exists vgmid vgmid' vlmid', vgmid = (((fst vg1) $+ (sig_name, varAss 1)), ((snd vg1) $+ (sig_name, varAss 1))) /\
-                match opt_callback with
-                    (*Context switch if n = 2*)
-                    | Some (f, n) =>  match n with
-                        | 2 => exists vgswitch vgreturn vldump, vgswitch = (((fst vgmid) $+ (("current")%string, varAss 2)), snd vgmid) /\ runStmtDual fuel' vgswitch ($0) (assignCallMethodStmt None f args) vgreturn vldump
-                        /\ vgmid' = (((fst vgreturn) $+ (("current")%string, varAss 1)), snd vgreturn) /\ vl1 = vlmid'
-                        | _ => runStmtDual fuel' vgmid vl1 (assignCallMethodStmt None f args) vgmid' vlmid'
-                        end
-                    | None => vgmid = vgmid' /\ vl1 = vlmid'
-                    end /\ match (fst vgmid') $? ("waiting_" ++ sig_name)%string with
-                        | Some (waitAss n b) => 
-                        (*Set current to 2 if n = 2 else leave it like that, then runStmt of the body, and switch back current to 1*)
-                            match n with
-                                | 2 => exists vgswitch vgreturn vldump, vgswitch = (((fst vgmid') $+ (("current")%string, varAss 2)), snd vgmid') /\ runStmtDual fuel' vgswitch ($0) b vgreturn vldump
-                                /\ vg2 = (((fst vgreturn) $+ (("current")%string, varAss 1)), snd vgreturn) /\ vlmid' = vl2
-                                | _ => runStmtDual fuel' vgmid' vlmid' b vg2 vl2
-                                end
-                        | _ => vgmid' = vg2 /\ vlmid' = vl2
-                        end
-            | skip => vg1 = vg2 /\ vl1 = vl2
-            end
-        | 2 => match st with
-            | varDeclStmt s e => exists n, n = interp2 e (snd vg1) vl1  /\ vl2 = (vl1 $+ (s, varAss n)) /\ vg1 = vg2
-            | ifStmt e s1 s2 => (exists r, r = interp2 e (snd vg1) vl1 /\ r <> 0 /\ runStmtDual fuel' vg1 vl1 s1 vg2 vl2) \/
-                (0 = interp2 e (snd vg1) vl1 /\ runStmtDual fuel' vg1 vl1 s2 vg2 vl2)
-            | whileStmt e s => (exists r vgmid vlmid, r = interp2 e (snd vg1) vl1 /\ r <> 0 /\ runStmtDual fuel' vg1 vl1 s vgmid vlmid 
-                /\ runStmtDual fuel' vgmid vlmid st vg2 vl2) \/ (0 = interp2 e (snd vg1) vl1 /\ vg1 = vg2 /\ vl1 = vl2)
-            | assignmentStmt s e => (vl1 $? s <> None /\ exists n, n = interp2 e (snd vg1) vl1 /\ vl2 = (vl1 $+ (s, varAss n)) /\ vg1 = vg2) \/
-                ((snd vg1) $? s <> None /\ vl1 $? s = None /\ exists n, n = interp2 e (snd vg1) vl1 /\ vg2 = (fst vg1, (snd vg1) $+ (s, varAss n)) /\ vl1 = vl2)
-            | awaitStmt sig_name => vg1 = vg2 /\ vl1 = vl2
-            | sequence s1 s2 => match s1 with
-                | awaitStmt sig_name => (exists r, (interp (Var sig_name) (fst vg1)) = r  /\ r <> 0 /\ runStmtDual fuel' vg1 vl1 s2 vg2 vl2 ) \/ 
-                ((interp (Var sig_name) (fst vg1) = 0) /\ vg2 = (((fst vg1) $+ (("waiting_" ++ sig_name)%string, waitAss 1 s2)), ((snd vg1) $+ (("waiting_" ++ sig_name)%string, waitAss 1 s2))))
-                | _ => exists vgmid vlmid, runStmtDual fuel' vg1 vl1 s1 vgmid vlmid /\ runStmtDual fuel' vgmid vlmid s2 vg2 vl2
-                end
-            (*The n is the program number of the program containing the fuction, refering to the index of the valuation to read to get the function*)
-            (*Note : We could just context switch before *)
-            | assignCallMethodStmt ret method_name args =>
-                match (snd vg1) $? method_name with 
-                | Some (methodAss name_args found_ret found_body) => 
-                    exists vlmid,
-                    runStmtDual fuel' vg1
-                    (fold_left 
-                        (fun (acc: valuation) (arg_argname: expr * string) => 
-                            (acc $+ ((snd arg_argname), varAss (interp2 (fst arg_argname) (snd vg1) vl1)))
-                        ) 
-                        (combine args name_args) ($0)) 
-                    found_body vg2 vlmid
-                    /\ match ret, found_ret with
-                        | Some s_ret, Some s_found_ret =>  (exists r, interp (Var s_found_ret) vlmid = r /\ vl2 = vl1 $+ (s_ret, varAss r))
-                        | Some _, None => False
-                        | None, _ => vl2 = vlmid
-                        end
-                | _ => False
-                end
-            | emitSignalStmt sig_name opt_callback args => exists vgmid vgmid' vlmid', vgmid = (((fst vg1) $+ (sig_name, varAss 1)), ((snd vg1) $+ (sig_name, varAss 1))) /\
-                match opt_callback with
-                    | Some (f, n) =>  match n with
-                        | 1 => exists vgswitch vgreturn vldump, vgswitch = (((fst vgmid) $+ (("current")%string, varAss 1)), snd vgmid) /\ runStmtDual fuel' vgswitch ($0) (assignCallMethodStmt None f args) vgreturn vldump
-                        /\ vgmid' = (((fst vgreturn) $+ (("current")%string, varAss 2)), snd vgreturn)
-                        | _ => runStmtDual fuel' vgmid vl1 (assignCallMethodStmt None f args) vgmid' vlmid'
-                        end
-                    | None => vgmid = vgmid' /\ vl1 = vlmid'
-                    end /\ match (fst vgmid') $? ("waiting_" ++ sig_name)%string with
-                        | Some (waitAss n b) => 
-                        (*Set current to 1 if n = 1 else leave it like that, then runStmt of the body, and switch back current to 2*)
-                            match n with
-                                | 1 => exists vgswitch vgreturn vldump, vgswitch = (((fst vgmid') $+ (("current")%string, varAss 1)), snd vgmid') /\ runStmtDual fuel' vgswitch ($0) b vgreturn vldump
-                                /\ vg2 = (((fst vgreturn) $+ (("current")%string, varAss 2)), snd vgreturn) /\ vlmid' = vl2
-                                | _ => runStmtDual fuel' vgmid' vlmid' b vg2 vl2
-                                end
-                        | _ => vgmid' = vg2 /\ vlmid' = vl2
-                        end
-            | skip => vg1 = vg2 /\ vl1 = vl2
-            end
-        | _ => False
-        end
-    end.
-
-(*NOTE / TODO : A chaque fois on écrit les waiting et les emitted dans les deux valuations mais en pratique on lit toujours dans la 1
-Aussi, on peut pas avoir 2 signaux du même nom dans deux programmes différents, mais ça y'a pas le choix sauf en mettant des nombres random*)
-    (*On suppose que quand on runDual 2 programmes, on donne une valuation qui contient déjà une entrée pour "current", qui est 1 si on run A, et 2 si on run B*)
-Fixpoint runDual (fuel: nat) (v1: valuation * valuation) (dA: topLevelDecl) (dB: topLevelDecl) (v2: valuation * valuation): Prop:=
-    match fuel with
-    | O => False
-    | S fuel' =>
-        (*Arbitrary choice to put current in fst and not snd*)
-        match interp (Var "current") (fst v1) with
-        | 1 => match dA with
-            | classVarDecl s e => exists n, n = interp e (fst v1)  /\ v2 = (((fst v1) $+ (s, varAss n)), snd v1)
-            | methodDecl s l ret st => v2 = (((fst v1) $+ (s, methodAss l ret st)), snd v1)
-            | readyDecl st => exists vl2, runStmtDual fuel' v1 ($0) st v2 vl2
-            | processDecl st1 => match dB with
-                | processDecl st2 => exists vmid vmid' vl2 vl2', runStmtDual fuel' v1 ($0) st1 vmid vl2 /\ runStmtDual fuel' vmid ($0) st2 vmid' vl2' /\ runDual fuel' vmid' dA dB v2 (*runStmt process A puis B, puis run infini*)
-                | EndDecl => run fuel' (fst v1) dA (fst v2) (*runStmt process A, puis run infini*)(*Quid de snd v2, si B await A dans son ready, il faut pouvoir l'appeler avec la bonne valuation*)
-                | _ => exists vmid, vmid = (((fst v1) $+ (("current")%string, varAss 2)), snd v1) /\ runDual fuel' vmid dA dB v2
-                end
-            | SequenceDecl d1 d2 => exists vmid, runDual fuel' v1 d1 dB vmid /\ runDual fuel' vmid d2 dB v2
-            | EndDecl => match dB with (*If B process : runStmt B + run B infini, else juste run B infini*)
-                                        (*If B EndDecl, v1 = v2 pour finir l'execution*)
-                | processDecl st2 => exists vmid vmid' vl2, vmid = (((fst v1) $+ (("current")%string, varAss 2)), snd v1) /\ runStmtDual fuel' vmid ($0) st2 vmid' vl2 /\ runDual fuel' vmid' dA dB v2
-                | EndDecl => v1 = v2
-                | _ => exists vmid, vmid = (((fst v1) $+ (("current")%string, varAss 2)), snd v1) /\ runDual fuel' vmid dA dB v2
-                end
-        
-            end 
-        | 2 => match dB with
-            | classVarDecl s e => exists n, n = interp e (snd v1)  /\ v2 = (fst v1, ((snd v1) $+ (s, varAss n)))
-            | methodDecl s l ret st => v2 = (fst v1, ((snd v1) $+ (s, methodAss l ret st)))
-            | readyDecl st => exists vl2, runStmtDual fuel' v1 ($0) st v2 vl2
-            | processDecl st => exists vmid, vmid = (((fst v1) $+ (("current")%string, varAss 1)), snd v1) /\ runDual fuel' vmid dA dB v2
-            | SequenceDecl d1 d2 => exists vmid, runDual fuel' v1 dA d1 vmid /\ runDual fuel' vmid dA d2 v2 
-            | EndDecl => exists vmid, vmid = (((fst v1) $+ (("current")%string, varAss 1)), snd v1) /\ runDual fuel' vmid dA dB v2
-            end 
-        | _ => False
-        end
-    end. *)
